@prefix : <https://w3id.org/todo/tododt#> .
@prefix owl: <http://www.w3.org/2002/07/owl#> .
@prefix rdf: <http://www.w3.org/1999/02/22-rdf-syntax-ns#> .
@prefix xml: <http://www.w3.org/XML/1998/namespace> .
@prefix xsd: <http://www.w3.org/2001/XMLSchema#> .
@prefix rdfs: <http://www.w3.org/2000/01/rdf-schema#> .
@base <https://w3id.org/todo/tododt> .

<https://w3id.org/todo/tododt> rdf:type owl:Ontology ;
                                <http://creativecommons.org/ns#license> "http://purl.org/NET/rdflicense/cc-by4.0" ;
                                <http://purl.org/dc/terms/contributor> "Izaskun Fernández (Tekniker) <mailto:izaskun.fernandez@tekniker.es>" ;
                                <http://purl.org/dc/terms/created> "2020-04-21T00:00:00"^^xsd:dateTime ;
                                <http://purl.org/dc/terms/creator> "Cristina Aceta (Tekniker) <mailto:cristina.aceta@tekniker.es>" ;
                                <http://purl.org/dc/terms/description> "Module for dialogue tracing." ;
                                <http://purl.org/dc/terms/issued> ""^^xsd:dateTime ;
                                <http://purl.org/dc/terms/modified> "2021-03-08T16:00:00"^^xsd:dateTime ;
                                <http://purl.org/dc/terms/title> "TODODT: Dialogue Tracing Module for Task-Oriented Dialogue management Ontology (TODO)" ;
                                <http://purl.org/vocab/vann/preferredNamespacePrefix> "tododt" ;
                                <http://purl.org/vocab/vann/preferredNamespaceUri> "" ;
                                owl:priorVersion "" ;
                                owl:versionInfo "1.0.0" .

#################################################################
#    Annotation properties
#################################################################

###  http://creativecommons.org/ns#license
<http://creativecommons.org/ns#license> rdf:type owl:AnnotationProperty .


###  http://purl.org/dc/terms/bibliographicCitation
<http://purl.org/dc/terms/bibliographicCitation> rdf:type owl:AnnotationProperty .


###  http://purl.org/dc/terms/contributor
<http://purl.org/dc/terms/contributor> rdf:type owl:AnnotationProperty .


###  http://purl.org/dc/terms/created
<http://purl.org/dc/terms/created> rdf:type owl:AnnotationProperty .


###  http://purl.org/dc/terms/creator
<http://purl.org/dc/terms/creator> rdf:type owl:AnnotationProperty .


###  http://purl.org/dc/terms/description
<http://purl.org/dc/terms/description> rdf:type owl:AnnotationProperty .


###  http://purl.org/dc/terms/issued
<http://purl.org/dc/terms/issued> rdf:type owl:AnnotationProperty .


###  http://purl.org/dc/terms/modified
<http://purl.org/dc/terms/modified> rdf:type owl:AnnotationProperty .


###  http://purl.org/dc/terms/title
<http://purl.org/dc/terms/title> rdf:type owl:AnnotationProperty .


###  http://purl.org/vocab/vann/preferredNamespacePrefix
<http://purl.org/vocab/vann/preferredNamespacePrefix> rdf:type owl:AnnotationProperty .


###  http://purl.org/vocab/vann/preferredNamespaceUri
<http://purl.org/vocab/vann/preferredNamespaceUri> rdf:type owl:AnnotationProperty .


###  http://www.w3.org/2002/07/owl#versionIRI
owl:versionIRI rdf:type owl:AnnotationProperty .


###  http://www.w3.org/2003/06/sw-vocab-status/ns#term_status
<http://www.w3.org/2003/06/sw-vocab-status/ns#term_status> rdf:type owl:AnnotationProperty .


###  http://www.w3.org/2004/02/skos/core#example
<http://www.w3.org/2004/02/skos/core#example> rdf:type owl:AnnotationProperty .


#################################################################
#    Datatypes
#################################################################

###  http://www.w3.org/2001/XMLSchema#time
xsd:time rdf:type rdfs:Datatype .


#################################################################
#    Object Properties
#################################################################

###  https://w3id.org/todo/tododt#hasSecondaryDialogue
:hasSecondaryDialogue rdf:type owl:ObjectProperty ,
                               owl:TransitiveProperty ;
                      rdfs:comment "Establishes the SecondaryDialogue corresponding to a DialogueTrace." ;
                      rdfs:isDefinedBy "https://w3id.org/todo/tododt#" ;
                      rdfs:label "hasSecondaryDialogue" ;
                      <http://www.w3.org/2003/06/sw-vocab-status/ns#term_status> "stable" .


###  https://w3id.org/todo/tododt#hasSystemRequest
:hasSystemRequest rdf:type owl:ObjectProperty ;
                  rdfs:comment "Establishes the SystemRequest corresponding to a SecondaryDialogueTrace." ;
                  rdfs:isDefinedBy "https://w3id.org/todo/tododt#" ;
                  rdfs:label "hasSystemRequest" ;
                  <http://www.w3.org/2003/06/sw-vocab-status/ns#term_status> "stable" .


###  https://w3id.org/todo/tododt#hasUserRequest
:hasUserRequest rdf:type owl:ObjectProperty ;
                rdfs:comment "Establishes the UserRequest corresponding to a DialogueTrace." ;
                rdfs:isDefinedBy "https://w3id.org/todo/tododt#" ;
                rdfs:label "hasUserRequest" ;
                <http://www.w3.org/2003/06/sw-vocab-status/ns#term_status> "stable" .


###  https://w3id.org/todo/tododt#hasUserResponse
:hasUserResponse rdf:type owl:ObjectProperty ;
                 rdfs:comment "Establishes the UserResponse corresponding to a SecondaryDialogueTrace." ;
                 rdfs:isDefinedBy "https://w3id.org/todo/tododt#" ;
                 rdfs:label "hasUserResponse" ;
                 <http://www.w3.org/2003/06/sw-vocab-status/ns#term_status> "stable" .


#################################################################
#    Data properties
#################################################################

###  https://w3id.org/todo/tododt#currentValue
:currentValue rdf:type owl:DatatypeProperty ;
              rdfs:comment "When asking the user for a specific information, the information currently asked to the user." ;
              rdfs:isDefinedBy "https://w3id.org/todo/tododt#" ;
              rdfs:label "currentValue" ;
              <http://www.w3.org/2003/06/sw-vocab-status/ns#term_status> "stable" ;
              <http://www.w3.org/2004/02/skos/core#example> """UserReq: \"I want to go to the room\"

possibleValue \"room1\"
possibleValue \"room2\"

SystemReq: \"Do you want to go to {room1}?\" (currentValue: room1); \"Do you want to go to {room2}? (currentValue: room2)\""""@en ,
                                                            """UserReq: \"Quiero ir a la sala\"

possibleValue \"sala1\"
possibleValue \"sala2\"

System Req: \"¿Quieres ir a la {sala1}?\" (currentValue: sala1); \"¿Quieres ir a la {sala2}? (currentValue: sala2)\""""@en .


###  https://w3id.org/todo/tododt#dateTime
:dateTime rdf:type owl:DatatypeProperty ;
          rdfs:range xsd:dateTime ;
          rdfs:comment "Sets a timestamp to a DialogueTrace." ;
          rdfs:isDefinedBy "https://w3id.org/todo/tododt#" ;
          rdfs:label "dateTime" ;
          <http://www.w3.org/2003/06/sw-vocab-status/ns#term_status> "stable" .


###  https://w3id.org/todo/tododt#dialStatus
:dialStatus rdf:type owl:DatatypeProperty ;
            rdfs:range [ rdf:type rdfs:Datatype ;
                         owl:oneOf [ rdf:type rdf:List ;
                                     rdf:first "closed" ;
                                     rdf:rest [ rdf:type rdf:List ;
                                                rdf:first "open" ;
                                                rdf:rest rdf:nil
                                              ]
                                   ]
                       ] ;
            rdfs:comment "Sets whether a Dialogue/SecondaryDialogue has finished (closed) or not (open)." ;
            rdfs:isDefinedBy "https://w3id.org/todo/tododt#" ;
            rdfs:label "dialStatus" ;
            <http://www.w3.org/2003/06/sw-vocab-status/ns#term_status> "stable" .


###  https://w3id.org/todo/tododt#dialogueStep
:dialogueStep rdf:type owl:DatatypeProperty ;
              rdfs:comment "Used to control which step is performing the current Dialogue." ;
              rdfs:isDefinedBy "https://w3id.org/todo/tododt#" ;
              rdfs:label "dialogueStep" ;
              <http://www.w3.org/2003/06/sw-vocab-status/ns#term_status> "stable" .


###  https://w3id.org/todo/tododt#finishDateTime
:finishDateTime rdf:type owl:DatatypeProperty ;
                rdfs:subPropertyOf :dateTime ;
                rdfs:comment "Sets a finish timestamp to a DialogueTrace." ;
                rdfs:isDefinedBy "https://w3id.org/todo/tododt#" ;
                rdfs:label "finishDateTime" ;
                <http://www.w3.org/2003/06/sw-vocab-status/ns#term_status> "stable" .


###  https://w3id.org/todo/tododt#initDateTime
:initDateTime rdf:type owl:DatatypeProperty ;
              rdfs:subPropertyOf :dateTime ;
              rdfs:comment "Sets a start timestamp to a DialogueTrace." ;
              rdfs:isDefinedBy "https://w3id.org/todo/tododt#" ;
              rdfs:label "initDateTime" ;
              <http://www.w3.org/2003/06/sw-vocab-status/ns#term_status> "stable" .


###  https://w3id.org/todo/tododt#possibleValue
:possibleValue rdf:type owl:DatatypeProperty ;
               rdfs:comment "When asking the user for a specific information, the possible values of that information to be asked to the user." ;
               rdfs:isDefinedBy "https://w3id.org/todo/tododt#" ;
               rdfs:label "possibleValue" ;
               <http://www.w3.org/2003/06/sw-vocab-status/ns#term_status> "stable" ;
               <http://www.w3.org/2004/02/skos/core#example> """UserReq: \"I want to go to the room\"

possibleValue \"room1\"
possibleValue \"room2\"

SystemReq: \"Do you want to go to {room1}?\"; \"Do you want to go to {room2}?\""""@en ,
                                                             """UserReq: \"Quiero ir a la sala\"

possibleValue \"sala1\"
possibleValue \"sala2\"

System Req: \"¿Quieres ir a la {sala1}?\"; \"¿Quieres ir a la {sala2}?\""""@es .


###  https://w3id.org/todo/tododt#text
:text rdf:type owl:DatatypeProperty ;
      rdfs:comment "String that corresponds to a transcribed command by an user or the fully constructed outputSentence directed to the user." ;
      rdfs:isDefinedBy "https://w3id.org/todo/tododt#" ;
      rdfs:label "text" ;
      <http://www.w3.org/2003/06/sw-vocab-status/ns#term_status> "stable" .


###  https://w3id.org/todo/tododt#verb
:verb rdf:type owl:DatatypeProperty ;
      rdfs:comment "Key element classified as \"verb\"/\"action\"." ;
      rdfs:isDefinedBy "https://w3id.org/todo/tododt#" ;
      rdfs:label "verb" ;
      <http://www.w3.org/2003/06/sw-vocab-status/ns#term_status> "stable" .


#################################################################
#    Classes
#################################################################

###  https://w3id.org/todo/tododt#ContentUserResponseTrace
:ContentUserResponseTrace rdf:type owl:Class ;
                          rdfs:subClassOf :UserResponseTrace ;
                          owl:disjointWith :YesNoUserResponseTrace ;
                          rdfs:comment "Element that leaves a record of the User Responses performed throughout the dialogue process. These responses provide specific information, as a response for a ContentRequest."@en ;
                          rdfs:isDefinedBy "https://w3id.org/todo/tododt#" ;
                          rdfs:label "ContentUserResponseTrace" ;
                          <http://www.w3.org/2003/06/sw-vocab-status/ns#term_status> "stable" ;
                          <http://www.w3.org/2004/02/skos/core#example> "Content User Response: The error code is 412."@en .


###  https://w3id.org/todo/tododt#DialogueProcessTrace
:DialogueProcessTrace rdf:type owl:Class ;
                      rdfs:subClassOf [ rdf:type owl:Restriction ;
                                        owl:onProperty :hasSecondaryDialogue ;
                                        owl:someValuesFrom :SecondaryDialogueTrace
                                      ] ,
                                      [ rdf:type owl:Restriction ;
                                        owl:onProperty :dialStatus ;
                                        owl:qualifiedCardinality "1"^^xsd:nonNegativeInteger ;
                                        owl:onDataRange [ rdf:type rdfs:Datatype ;
                                                          owl:oneOf [ rdf:type rdf:List ;
                                                                      rdf:first "close" ;
                                                                      rdf:rest [ rdf:type rdf:List ;
                                                                                 rdf:first "open" ;
                                                                                 rdf:rest rdf:nil
                                                                               ]
                                                                    ]
                                                        ]
                                      ] ,
                                      [ rdf:type owl:Restriction ;
                                        owl:onProperty :finishDateTime ;
                                        owl:qualifiedCardinality "1"^^xsd:nonNegativeInteger ;
                                        owl:onDataRange xsd:dateTime
                                      ] ,
                                      [ rdf:type owl:Restriction ;
                                        owl:onProperty :initDateTime ;
                                        owl:qualifiedCardinality "1"^^xsd:nonNegativeInteger ;
                                        owl:onDataRange xsd:dateTime
                                      ] ;
                      rdfs:comment "Element that leaves a record of the dialogues performed throughout the dialogue process." ;
                      rdfs:isDefinedBy "https://w3id.org/todo/tododt#" ;
                      rdfs:label "DialogueProcessTrace" ;
                      <http://www.w3.org/2003/06/sw-vocab-status/ns#term_status> "stable" .


###  https://w3id.org/todo/tododt#DialogueTrace
:DialogueTrace rdf:type owl:Class ;
               rdfs:subClassOf :DialogueProcessTrace ,
                               [ rdf:type owl:Restriction ;
                                 owl:onProperty :hasUserRequest ;
                                 owl:someValuesFrom :UserRequestTrace
                               ] ,
                               [ rdf:type owl:Restriction ;
                                 owl:onProperty :dialogueStep ;
                                 owl:qualifiedCardinality "1"^^xsd:nonNegativeInteger ;
                                 owl:onDataRange xsd:string
                               ] ;
               rdfs:comment "Element that leaves a record of the dialogues performed." ;
               rdfs:isDefinedBy "https://w3id.org/todo/tododt#" ;
               rdfs:label "DialogueTrace" ;
               <http://www.w3.org/2003/06/sw-vocab-status/ns#term_status> "stable" .


###  https://w3id.org/todo/tododt#NoUserResponse
:NoUserResponse rdf:type owl:Class ;
                rdfs:subClassOf :YesNoUserResponseTrace ;
                rdfs:comment "Element that leaves a record of the User Responses performed throughout the dialogue process. These responses correspond to a negative polarity."@en ;
                rdfs:isDefinedBy "https://w3id.org/todo/tododt#" ;
                rdfs:label "NoUserResponse" ;
                <http://www.w3.org/2003/06/sw-vocab-status/ns#term_status> "stable" ;
                <http://www.w3.org/2004/02/skos/core#example> "No User Responses: No, Never, Not at all"@en .


###  https://w3id.org/todo/tododt#NullUserResponseTrace
:NullUserResponseTrace rdf:type owl:Class ;
                       rdfs:subClassOf :UserResponseTrace ;
                       rdfs:comment "Response that does not represent a value that can be classified as ContentResponse or YesNoResponse."@en ;
                       rdfs:isDefinedBy "https://w3id.org/todo/tododt#" ;
                       rdfs:label "NullUserResponseTrace" ;
                       <http://www.w3.org/2003/06/sw-vocab-status/ns#term_status> "stable" ;
                       <http://www.w3.org/2004/02/skos/core#example> "Null User Response: I don't know."@en .


###  https://w3id.org/todo/tododt#SecondaryDialogueTrace
:SecondaryDialogueTrace rdf:type owl:Class ;
                        rdfs:subClassOf :DialogueProcessTrace ,
                                        [ rdf:type owl:Restriction ;
                                          owl:onProperty :hasSystemRequest ;
                                          owl:someValuesFrom :SystemRequestTrace
                                        ] ,
                                        [ rdf:type owl:Restriction ;
                                          owl:onProperty :hasUserResponse ;
                                          owl:someValuesFrom :UserResponseTrace
                                        ] ,
                                        [ rdf:type owl:Restriction ;
                                          owl:onProperty :text ;
                                          owl:qualifiedCardinality "1"^^xsd:nonNegativeInteger ;
                                          owl:onDataRange xsd:string
                                        ] ;
                        rdfs:comment "Element that leaves a record of the secondary dialogues performed." ;
                        rdfs:isDefinedBy "https://w3id.org/todo/tododt#" ;
                        rdfs:label "SecondaryDialogueTrace" ;
                        <http://www.w3.org/2003/06/sw-vocab-status/ns#term_status> "stable" .


###  https://w3id.org/todo/tododt#SystemRequestTrace
:SystemRequestTrace rdf:type owl:Class ;
                    rdfs:subClassOf :SystemStepTrace ;
                    rdfs:comment "Element that leaves a record of the SystemRequests performed throughout the dialogue process." ;
                    rdfs:isDefinedBy "https://w3id.org/todo/tododt#" ;
                    rdfs:label "SystemRequestTrace" ;
                    <http://www.w3.org/2003/06/sw-vocab-status/ns#term_status> "stable" .


###  https://w3id.org/todo/tododt#SystemResponseTrace
:SystemResponseTrace rdf:type owl:Class ;
                     rdfs:subClassOf :SystemStepTrace ;
                     rdfs:comment "Element that leaves a record of the SystemResponses performed throughout the dialogue process." ;
                     rdfs:isDefinedBy "https://w3id.org/todo/tododt#" ;
                     rdfs:label "SystemResponseTrace" ;
                     <http://www.w3.org/2003/06/sw-vocab-status/ns#term_status> "stable" .


###  https://w3id.org/todo/tododt#SystemStepTrace
:SystemStepTrace rdf:type owl:Class ;
                 rdfs:comment "Element that leaves a record of the SystemSteps performed throughout the dialogue process." ;
                 rdfs:isDefinedBy "https://w3id.org/todo/tododt#" ;
                 rdfs:label "SystemStepTrace" ;
                 <http://www.w3.org/2003/06/sw-vocab-status/ns#term_status> "stable" .


###  https://w3id.org/todo/tododt#UserRequestTrace
:UserRequestTrace rdf:type owl:Class ;
                  rdfs:subClassOf :UserStepTrace ;
                  owl:disjointWith :UserResponseTrace ;
                  rdfs:comment "Element that leaves a record of the User Requests performed throughout the dialogue process."@en ;
                  rdfs:isDefinedBy "https://w3id.org/todo/tododt#" ;
                  rdfs:label "UserRequestTrace" ;
                  <http://www.w3.org/2003/06/sw-vocab-status/ns#term_status> "stable" .


###  https://w3id.org/todo/tododt#UserResponseTrace
:UserResponseTrace rdf:type owl:Class ;
                   rdfs:subClassOf :UserStepTrace ;
                   rdfs:comment "Element that leaves a record of the User Responses performed throughout the dialogue process."@en ;
                   rdfs:isDefinedBy "https://w3id.org/todo/tododt#" ;
                   rdfs:label "UserResponseTrace" ;
                   <http://www.w3.org/2003/06/sw-vocab-status/ns#term_status> "stable" .


###  https://w3id.org/todo/tododt#UserStepTrace
:UserStepTrace rdf:type owl:Class ;
               rdfs:subClassOf [ rdf:type owl:Restriction ;
                                 owl:onProperty :text ;
                                 owl:qualifiedCardinality "1"^^xsd:nonNegativeInteger ;
                                 owl:onDataRange xsd:string
                               ] ;
               rdfs:comment "Element that leaves a record of the user steps (requests and responses) performed throughout the dialogue process." ;
               rdfs:isDefinedBy "https://w3id.org/todo/tododt#" ;
               rdfs:label "UserStepTrace" ;
               <http://www.w3.org/2003/06/sw-vocab-status/ns#term_status> "stable" .


###  https://w3id.org/todo/tododt#YesNoUserResponseTrace
:YesNoUserResponseTrace rdf:type owl:Class ;
                        rdfs:subClassOf :UserResponseTrace ;
                        rdfs:comment "Element that leaves a record of the User Responses performed throughout the dialogue process. These responses correspond to a positive or negative polarity."@en ;
                        rdfs:isDefinedBy "https://w3id.org/todo/tododt#" ;
                        rdfs:label "YesNoUserResponseTrace" ;
                        <http://www.w3.org/2003/06/sw-vocab-status/ns#term_status> "stable" ;
                        <http://www.w3.org/2004/02/skos/core#example> """YesNo User Responses:

- Yes, OK

- No, Not at all"""@en .


###  https://w3id.org/todo/tododt#YesUserResponse
:YesUserResponse rdf:type owl:Class ;
                 rdfs:subClassOf :YesNoUserResponseTrace ;
                 rdfs:comment "Element that leaves a record of the User Responses performed throughout the dialogue process. These responses correspond to a positive polarity."@en ;
                 rdfs:isDefinedBy "https://w3id.org/todo/tododt#" ;
                 rdfs:label "YesUserResponse" ;
                 <http://www.w3.org/2003/06/sw-vocab-status/ns#term_status> "stable" ;
                 <http://www.w3.org/2004/02/skos/core#example> "Yes User Responses: Yes, OK"@en .


###  Generated by the OWL API (version 5.1.14) https://github.com/owlcs/owlapi/
